compiler/src/examples/end2endTests.v
@@ -1,0 +1,116 @@
+Require Import String.
+Require Import Coq.ZArith.ZArith.
+Require Import coqutil.Z.Lia.
+Require Import Coq.Lists.List. Import ListNotations.
+Require Import Coq.Logic.FunctionalExtensionality.
+Require Import riscv.Spec.Decode.
+Require Import riscv.Utility.Encode.
+Require Import riscv.Utility.Utility.
+Require Import coqutil.Word.LittleEndian.
+Require Import coqutil.Word.Properties.
+Require Import coqutil.Map.Interface.
+Require Import coqutil.Tactics.Tactics.
+Require Import riscv.Spec.Primitives.
+Require Import riscv.Spec.Machine.
+Require riscv.Platform.Memory.
+Require Import riscv.Spec.PseudoInstructions.
+Require Import riscv.Proofs.EncodeBound.
+Require Import riscv.Proofs.DecodeEncode.
+Require Import riscv.Platform.Run.
+Require Import riscv.Utility.MkMachineWidth.
+Require Import riscv.Utility.Monads. Import MonadNotations.
+Require Import riscv.Utility.runsToNonDet.
+Require Import coqutil.Datatypes.PropSet.
+Require Import riscv.Utility.MMIOTrace.
+Require Import riscv.Platform.RiscvMachine.
+Require Import riscv.Platform.MetricRiscvMachine.
+Require Import riscv.Spec.MetricPrimitives.
+Require Import compiler.RunInstruction.
+Require Import compiler.EventLoop.
+Require Import compiler.ForeverSafe.
+Require Import compiler.GoFlatToRiscv.
+
+
+Local Open Scope Z_scope.
+
+Section Test.
+
+  Context {M: Type -> Type}.
+  Context {W: Utility.Words}.
+
+  Context {Registers: map.map Register word}
+          {mem: map.map word byte}
+          {mm: Monad M}
+          {rvm: RiscvProgram M word}.
+
+  Context (KamiMachine: Type).
+
+  Context (instrMemSizeLg: Z).
+
+  (* common event between riscv-coq and Kami *)
+  Inductive Event: Type :=
+  | MMInputEvent(addr v: word)
+  | MMOutputEvent(addr v: word).
+
+  Context (kamiStep: KamiMachine -> KamiMachine -> list Event -> Prop).
+
+  Context (states_related: KamiMachine * list Event -> MetricRiscvMachine -> Prop).
+
+  Context {PRParams: PrimitivesParams M MetricRiscvMachine}.
+  Context {PR: MetricPrimitives PRParams}.
+
+  Inductive star{S E: Type}(R: S -> S -> list E -> Prop): S -> S -> list E -> Prop :=
+  | star_refl: forall (x: S),
+      star R x x nil
+  | star_step: forall (x y z: S) (t1 t2: list E),
+      R x y t1 ->
+      star R y z t2 ->
+      star R x z (t2 ++ t1).
+
+  (* something like this is being proved in processor/src/KamiRiscv.v *)
+  Hypothesis kamiStep_sound: forall (m1 m2: KamiMachine) (m1': MetricRiscvMachine)
+                                    (t t0: list Event) (post: MetricRiscvMachine -> Prop),
+      kamiStep m1 m2 t ->
+      states_related (m1, t0) m1' ->
+      mcomp_sat (run1 iset) m1' post ->
+      (* Either Kami doesn't proceed or riscv-coq simulates. *)
+      ((m1 = m2 /\ t = nil) (* <-- "t = nil" added *) \/
+       exists m2', states_related (m2, t ++ t0) m2' /\ post m2').
+
+  Lemma Return_tt_nop: forall comp m post,
+      mcomp_sat (comp;; Return tt) m post ->
+      mcomp_sat comp m post.
+  Proof.
+    Close Scope monad_scope.
+    intros. rewrite <- (right_identity comp).
+    replace Return with (fun _ : unit => Return tt); [assumption|].
+    extensionality x. destruct x. reflexivity.
+  Qed.
+
+  Lemma kamiMultiStep_sound: forall
+    (* inv could (and probably has to) be something like "runs to a safe state" *)
+    (inv: MetricRiscvMachine -> Prop)
+    (* could be instantiated with compiler.ForeverSafe.runsTo_safe1_inv *)
+    (inv_preserved: forall st, inv st -> mcomp_sat (run1 iset) st inv)
+    (m1 m2: KamiMachine) (t: list Event),
+      star kamiStep m1 m2 t ->
+      forall (m1': MetricRiscvMachine) (t0: list Event),
+      states_related (m1, t0) m1' ->
+      inv m1' ->
+      exists m2', states_related (m2, t ++ t0) m2' /\ inv m2'.
+  Proof.
+    intros ? ?.
+    induction 1; intros.
+    - exists m1'. split; assumption.
+    - pose proof kamiStep_sound as P.
+      specialize P with (1 := H) (2 := H1).
+      edestruct P as [Q | Q]; clear P.
+      + eapply inv_preserved. assumption.
+      + destruct Q. subst. rewrite List.app_nil_r.
+        eapply IHstar; eassumption.
+      + destruct Q as (m2' & Rel & Inv).
+        rewrite <- List.app_assoc.
+        eapply IHstar; eassumption.
+  Qed.
+
+End Test.
